Update, began refactor, tap at freshness

FreydSSA/Basic.lean
@@ -4,116 +4,7 @@ import Mathlib.Data.Set.Basic
 import Mathlib.Data.Set.Function
 import Mathlib.Init.Classical
 
-open List.«term_<+_»
-
-structure Var (ν : Type u) (α : Type v) : Type (max u v) where
-  name: ν
-  ty: α
-
-def Ctx (ν : Type u) (α : Type v) : Type (max u v) := List (Var ν α)
-
-inductive Ctx.Iso : Ctx ν α → Ctx ν' α → Prop
-  | nil : Ctx.Iso [] []
-  | cons : Ctx.Iso Γ Δ → Ctx.Iso (⟨n, a⟩::Γ) (⟨n', a⟩::Δ)
-
-theorem Ctx.Iso.cons'
-  : {x : Var ν α} → {x' : Var ν' α} → (hx: x.ty = x'.ty) → (h: Ctx.Iso Γ Δ)
-    → Ctx.Iso (x::Γ) (x'::Δ)
-  | ⟨_, _⟩, ⟨_, _⟩, rfl, h => Ctx.Iso.cons h
-
-inductive Ctx.HasVar {ν α : Type u} (A : α) : ℕ → Ctx ν α → Prop
-  | head : Ctx.HasVar A 0 (⟨n, A⟩::Γ)
-  | tail : Ctx.HasVar A n Γ → Ctx.HasVar A (n+1) (x::Γ)
-
-structure Ctx.Ix {ν α} (Γ : Ctx ν α) (A : α) : Type where
-  val : ℕ
-  hasVar : Ctx.HasVar A val Γ
-
-@[simp]
-def Ctx.names {ν α} (Γ : Ctx ν α): List ν
-  := Γ.map Var.name
-
-inductive Ctx.Fresh {ν α} (n : ν) : Ctx ν α → Prop
-  | nil : Ctx.Fresh n []
-  | cons {Γ x} : x.name ≠ n → Ctx.Fresh n Γ → Ctx.Fresh n (x::Γ)
-
-theorem Ctx.Fresh.head {ν α} {n} {y : Var ν α} {Γ : Ctx ν α}
-  : Ctx.Fresh n (y::Γ) → y.name ≠ n
-  | cons hxn _ => hxn
-
-theorem Ctx.Fresh.tail {ν α} {n} {y : Var ν α} {Γ : Ctx ν α}
-  : Ctx.Fresh n (y::Γ) → Ctx.Fresh n Γ
-  | cons _ hn => hn
-
-inductive Ctx.Wk {ν: Type u} {α: Type v} : Ctx ν α → Ctx ν α → Type (max u v)
-  | nil : Ctx.Wk [] []
-  | cons {Γ Δ} (x : Var ν α) : Ctx.Wk Γ Δ → Ctx.Wk (x::Γ) (x::Δ)
-  | skip {Γ Δ} : Ctx.Fresh x.name Δ → Ctx.Wk Γ Δ → Ctx.Wk (x::Γ) Δ
-
-theorem Ctx.Fresh.wk {ν α} {Γ Δ: Ctx ν α} {n: ν}: Fresh n Γ → Γ.Wk Δ → Fresh n Δ
-  | _, Wk.nil => nil
-  | cons hxn hn, Wk.cons _ h => cons hxn (hn.wk h)
-  | cons _ hn, Wk.skip _ h => hn.wk h
-
-def Ctx.Wk.comp {ν α} {Γ Δ Ξ : Ctx ν α} : Γ.Wk Δ → Δ.Wk Ξ → Γ.Wk Ξ
-  | nil, h => h
-  | cons x h, cons _ h' => cons x (h.comp h')
-  | cons _ h, skip hn h' => skip hn (h.comp h')
-  | skip hn h, h' => skip (hn.wk h') (h.comp h')
-
-theorem Ctx.Wk.allEq {ν α} {Γ Δ : Ctx ν α} (D D': Γ.Wk Δ): D = D'
-  := by induction D with
-  | nil => cases D'; rfl
-  | cons _ _ I => cases D' with
-    | cons => exact congrArg _ (I _)
-    | skip hxn => exact (hxn.head rfl).elim
-  | skip hxn _ I => cases D' with
-    | cons _ _ => exact (hxn.head rfl).elim
-    | skip h I' => exact congrArg _ (I I')
-
-def Ctx.Wk.refl {ν α} : (Γ : Ctx ν α) → Γ.Wk Γ
-  | [] => nil
-  | x::Γ => cons x (refl Γ)
-
-def Ctx.Wk.drop {ν α} : (Γ : Ctx ν α) → Γ.Wk []
-  | [] => nil
-  | _::Γ => skip Fresh.nil (drop Γ)
-
-inductive Ctx.Wk.Iso : {Γ Δ : Ctx ν α} → {Γ' Δ' : Ctx ν' α'} → Ctx.Wk Γ Δ → Ctx.Wk Γ' Δ' → Prop
-  | nil : Ctx.Wk.Iso nil nil
-  | cons : Ctx.Wk.Iso w w' → Ctx.Wk.Iso (cons h w) (cons h' w')
-  | skip : Ctx.Wk.Iso w w' → Ctx.Wk.Iso (skip h w) (skip h' w')
-
-theorem Ctx.Wk.iso_refl {Γ Δ : Ctx ν α} : (w: Γ.Wk Δ) → w.Iso w
-  | Wk.nil => Iso.nil
-  | Wk.cons h w => Iso.cons w.iso_refl
-  | Wk.skip h w => Iso.skip w.iso_refl
-
-theorem Ctx.Wk.Iso.refl {Γ Δ : Ctx ν α} : (w: Γ.Wk Δ) → w.Iso w
-  | Wk.nil => Iso.nil
-  | Wk.cons h w => Iso.cons w.iso_refl
-  | Wk.skip h w => Iso.skip w.iso_refl
-
-theorem Ctx.Wk.Iso.symm {Γ Δ : Ctx ν α} {Γ' Δ' : Ctx ν' α'} {w: Γ.Wk Δ} {w': Γ'.Wk Δ'}
-  : w.Iso w' → w'.Iso w
-  | Iso.nil => Iso.nil
-  | Iso.cons I => Iso.cons (I.symm)
-  | Iso.skip I => Iso.skip (I.symm)
-
-theorem Ctx.Wk.Iso.trans {Γ Δ : Ctx ν α} {Γ' Δ' : Ctx ν' α'} {Γ'' Δ'' : Ctx ν'' α''}
-  {w: Γ.Wk Δ} {w': Γ'.Wk Δ'} {w'': Γ''.Wk Δ''}
-  : w.Iso w' → w'.Iso w'' → w.Iso w''
-  | Iso.nil, Iso.nil => Iso.nil
-  | Iso.cons I, Iso.cons I' => Iso.cons (I.trans I')
-  | Iso.skip I, Iso.skip I' => Iso.skip (I.trans I')
-
-theorem Ctx.Wk.Iso.comp {Γ Δ Ξ : Ctx ν α} {Γ' Δ' Ξ' : Ctx ν' α}
-  {l: Γ.Wk Δ} {r: Δ.Wk Ξ} {l': Γ'.Wk Δ'} {r': Δ'.Wk Ξ'}
-  : l.Iso l' → r.Iso r' → (l.comp r).Iso (l'.comp r')
-  | Iso.nil, hr => hr
-  | Iso.cons Il, Iso.cons Ir => Iso.cons (Il.comp Ir)
-  | Iso.cons Il, Iso.skip Ir => Iso.skip (Il.comp Ir)
-  | Iso.skip Il, hr => Iso.skip (Il.comp hr)
+import FreydSSA.Ctx
 
 --TODO: antisymm...
 
@@ -133,7 +24,6 @@ instance : OfNat Purity 0 where
 instance : OfNat Purity 1 where
   ofNat := Purity.pure
 
---TODO: make into struct parameter?
 structure InstSet (α : Type u) : Type _ where
   Op : Purity → α → α → Type
   pure_to_impure : Op 1 a b → Op 0 a b
@@ -338,7 +228,7 @@ def Ctx.InjOn (ρ : ν → ν') (Γ : Ctx ν α) : Prop
   := Set.InjOn ρ { x : ν | x ∈ Γ.names }
 
 theorem Ctx.injOn_empty (ρ : ν → ν') : Ctx.InjOn ρ (@List.nil (Var ν α))
-  := λ _ hx => match hx with .
+  := λ _ hx => nomatch hx
 
 theorem Ctx.InjOn.tail {ρ: ν → ν'} {v} {Γ : Ctx ν α} (h: Ctx.InjOn ρ (v::Γ))
   : Ctx.InjOn ρ Γ
@@ -488,13 +378,13 @@ inductive InstSet.Body.Fresh {Φ : InstSet (Ty α)} (n: ν)
   | let2 {b: Φ.Body p (⟨x, A⟩::⟨y, B⟩::Γ) Δ} (e: Φ.Tm p Γ (Ty.pair A B)):
     b.Fresh n → (b.let2 e).Fresh n
 
-def InstSet.Body.Fresh.entry {Φ : InstSet (Ty α)} {Γ Δ : Ctx ν (Ty α)} {p}
+theorem InstSet.Body.Fresh.entry {Φ : InstSet (Ty α)} {Γ Δ : Ctx ν (Ty α)} {p}
   {b : Φ.Body p Γ Δ} {n} : b.Fresh n → Γ.Fresh n
   | nil _ h => h
   | let1 _ h => h.entry.tail
   | let2 _ h => h.entry.tail.tail
 
-def InstSet.Body.Fresh.exit {Φ : InstSet (Ty α)} {Γ Δ : Ctx ν (Ty α)} {p}
+theorem InstSet.Body.Fresh.exit {Φ : InstSet (Ty α)} {Γ Δ : Ctx ν (Ty α)} {p}
   {b : Φ.Body p Γ Δ} {n} : b.Fresh n → Δ.Fresh n
   | nil w h => h.wk w
   | let1 _ h => h.exit
@@ -546,19 +436,32 @@ theorem InstSet.Body.NotDef.iff_not_mem_defs {Φ: InstSet (Ty α)} {b: Φ.Body p
   : b.NotDef n ↔ n ∉ b.defs
   := ⟨not_mem_defs, of_not_mem_defs⟩
 
-def InstSet.Body.Fresh.notDef {Φ : InstSet (Ty α)} {Γ Δ : Ctx ν (Ty α)} {p}
+theorem InstSet.Body.Fresh.notDef {Φ : InstSet (Ty α)} {Γ Δ : Ctx ν (Ty α)} {p}
   {b : Φ.Body p Γ Δ} {n} : b.Fresh n → b.NotDef n
   | nil _ h => NotDef.nil _
   | let1 _ h => NotDef.let1 h.entry.head _ h.notDef
   | let2 _ h => NotDef.let2 h.entry.head h.entry.tail.head _ h.notDef
 
+theorem InstSet.Body.NotDef.toFresh {Φ: InstSet (Ty α)} {Γ Δ : Ctx ν (Ty α)} {p}
+  {b: Φ.Body p Γ Δ} {n} (hb: b.NotDef n) (hΓ: Γ.Fresh n): b.Fresh n
+  := by induction hb with
+  | _ =>
+    constructor
+    apply_assumption
+    repeat first | apply Ctx.Fresh.cons | assumption
+
 inductive InstSet.Body.SSA {Φ: InstSet (Ty α)}
   : {Γ Δ: Ctx ν (Ty α)} → Φ.Body p Γ Δ → Prop
   | nil {Γ Δ: Ctx ν (Ty α)} (h: Γ.Wk Δ): Body.SSA (Body.nil p h)
   | let1 {b: Φ.Body p (⟨x, A⟩::Γ) Δ}:
-    b.NotDef x → (e: Φ.Tm p Γ A) → b.SSA → (b.let1 e).SSA
+    Ctx.Fresh x Γ → (e: Φ.Tm p Γ A) → b.SSA → (b.let1 e).SSA
   | let2 {b: Φ.Body p (⟨x, A⟩::⟨y, B⟩::Γ) Δ}:
-    b.NotDef x → b.NotDef y → (e: Φ.Tm p Γ (Ty.pair A B)) → b.SSA → (b.let2 e).SSA
+      x ≠ y →
+      Ctx.Fresh x Γ →
+      Ctx.Fresh y Γ →
+      (e: Φ.Tm p Γ (Ty.pair A B)) →
+      b.SSA →
+      (b.let2 e).SSA
 
 def InstSet.Body.αSSA {Φ: InstSet (Ty α)} (b: Φ.Body p Γ Δ): Prop
   := ∃b' : Φ.Body p Γ Δ, b'.SSA ∧ b.Iso b'
@@ -582,79 +485,6 @@ structure InstSet.SSABody {Φ: InstSet (Ty α)} (p: Purity) (Γ Δ: Ctx ν (Ty �
 
 -- TODO: in particular, if ν is infinite (or actually, just > |b| + |Γ|), then every body from Γ to
 --Δ is in αSSA
-
-structure Label (ν : Type u) (α : Type v) extends Var ν α where
-  live : Ctx ν α
-
-structure Label.Wk (ℓ ℓ' : Label ν α) where
-  var : ℓ.toVar = ℓ'.toVar
-  live : ℓ.live.Wk ℓ'.live
-
-def Label.Wk.refl (ℓ : Label ν α) : ℓ.Wk ℓ := ⟨rfl, Ctx.Wk.refl _⟩
-
-def Label.Wk.comp {ℓ ℓ' ℓ'' : Label ν α} (w : ℓ.Wk ℓ') (w' : ℓ'.Wk ℓ'') : ℓ.Wk ℓ''
-  := ⟨w.var.trans w'.var, w.live.comp w'.live⟩
-
-abbrev Label.Wk.Iso {ℓ ℓ' ℓ'' ℓ''' : Label ν α} (w : ℓ.Wk ℓ') (w' : ℓ''.Wk ℓ''')
-  := w.live.Iso w'.live
-
-structure Label.Fresh (ℓ : Label ν α) (n : ν): Prop where
-  name : ℓ.name ≠ n
-  live : ℓ.live.Fresh n
-
-def LCtx (ν: Type u) (α: Type v) := List (Label ν α)
-
-inductive LCtx.Fresh {ν α} (n : ν) : LCtx ν α → Prop
-  | nil : LCtx.Fresh n []
-  | cons : ℓ.Fresh n → Fresh n L → Fresh n (ℓ::L)
-
-theorem LCtx.Fresh.head {ν α} {n} {ℓ : Label ν α} {L : LCtx ν α}
-  : LCtx.Fresh n (ℓ::L) → ℓ.Fresh n
-  | cons hxn _ => hxn
-
-theorem LCtx.Fresh.tail {ν α} {n} {ℓ : Label ν α} {L : LCtx ν α}
-  : LCtx.Fresh n (ℓ::L) → L.Fresh n
-  | cons _ h => h
-
-inductive LCtx.Wk {ν : Type u} {α : Type v} : LCtx ν α → LCtx ν α → Type (max u v)
-  | nil : Wk [] []
-  | cons {ℓ ℓ' : Label ν α} : ℓ.Wk ℓ' → Wk L K → Wk (ℓ::L) (ℓ'::K)
-  | skip (ℓ : Label ν α) : Wk L K → Wk L (ℓ::K) --TODO: freshness?
-
-def LCtx.Wk.comp {L K M : LCtx ν α} : L.Wk K → K.Wk M → L.Wk M
-  | Wk.nil, w => w
-  | Wk.cons h w, Wk.cons h' w' => Wk.cons (h.comp h') (w.comp w')
-  | Wk.skip _ w, Wk.cons h w' => Wk.skip _ (w.comp w')
-  | w, Wk.skip ℓ w' => Wk.skip _ (w.comp w')
-
-inductive LCtx.Wk.Iso : {L K : LCtx ν α} → {L' K' : LCtx ν' α'} → Wk L K → Wk L' K' → Prop
-  | nil : Iso nil nil
-  | cons : h.Iso h' → Iso w w' → Iso (cons h w) (cons h' w')
-  | skip (ℓ ℓ') : Iso w w' → Iso (skip ℓ w) (skip ℓ' w')
-
-theorem LCtx.Wk.Iso.refl {L K : LCtx ν α} : (w: L.Wk K) → w.Iso w
-  | Wk.nil => nil
-  | Wk.cons h w => cons h.live.iso_refl (refl w)
-  | Wk.skip _ w => skip _ _ (refl w)
-
-theorem LCtx.Wk.Iso.symm {L K : LCtx ν α} {L' K' : LCtx ν' α'}
-  {w: L.Wk K} {w': L'.Wk K'} : (h: w.Iso w') → w'.Iso w
-  | nil => nil
-  | cons h w => cons h.symm w.symm
-  | skip _ _ w => skip _ _ w.symm
-
-theorem LCtx.Wk.Iso.trans {L K : LCtx ν α} {L' K' : LCtx ν' α'} {L'' K'' : LCtx ν'' α''}
-  {w: L.Wk K} {w': L'.Wk K'} {w'': L''.Wk K''} : (h: w.Iso w') → (h': w'.Iso w'') → w.Iso w''
-  | nil, nil => nil
-  | cons h w, cons h' w' => cons (h.trans h') (w.trans w')
-  | skip _ _ w, skip _ _ w' => skip _ _ (w.trans w')
-
-theorem LCtx.Wk.Iso.comp {L K M : LCtx ν α} {L' K' M' : LCtx ν' α'}
-  {l: L.Wk K} {r: K.Wk M} {l': L'.Wk K'} {r': K'.Wk M'}
-  (hl: l.Iso l') (hr: r.Iso r'): (l.comp r).Iso (l'.comp r') := by
-  induction hr generalizing L
-  <;> cases hl
-  <;> repeat first | apply Ctx.Wk.Iso.comp | apply_assumption | constructor
 
 inductive InstSet.Terminator
   (Φ : InstSet (Ty α)) (Γ : Ctx ν (Ty α)) (L : LCtx ν (Ty α))
